restructure for win_count

theories/Compositional_Structures/Basic_Modules/Component_Types/Social_Choice_Types/Counting_Functions_Code.thy
@@ -32,8 +32,8 @@ definition index_mon :: "'a Preference_List \<Rightarrow> 'a \<Rightarrow> nat n
   (\<lambda>(i, found). (i < (length ballot) \<and> \<not>found)) 
       (\<lambda>(i,_). do {
       ASSERT (i < (length ballot));
-      let xi = ballot!i; \<comment> \<open>It's not trivial to show that \<open>i\<close> is in range\<close>
-      if a=xi then
+      let (c) = (ballot!i);
+      if (a = c) then
         RETURN (i,True)
       else
         RETURN (i+1,False)
@@ -82,16 +82,22 @@ next
     by (metis antisym index_le_size le_neq_implies_less order_trans)
 qed
 
+lemma index_mon_refine:
+  shows "(index_mon, (\<lambda> ballot a. (RETURN (List_Index.index ballot a))))\<in> Id \<rightarrow> Id \<rightarrow> \<langle>Id\<rangle>nres_rel"
+  apply (refine_vcg index_mon_correct)
+  apply simp
+  done
+
 definition rank_mon :: "'a Preference_List \<Rightarrow> 'a \<Rightarrow> nat nres" where
   "rank_mon ballot a \<equiv> do {
     i \<leftarrow> (index_mon ballot a);
     RETURN (if (i = length ballot) then 0 else (i + 1))
-  }"                          
+  }"       
 
 
 lemma rank_mon_correct: "rank_mon ballot a \<le> SPEC (\<lambda> r. r = rank_l ballot a)"
   unfolding rank_mon_def
-proof (refine_vcg, clarsimp_all, safe)
+proof (refine_vcg, (simp_all add: rankdef), safe)
   assume mem: "List.member ballot a"
   from this have "index ballot a \<noteq> length ballot"
     by (simp add: in_set_member index_size_conv)
@@ -106,6 +112,13 @@ next
     using index_mon_correct
     by (metis singleton_conv)
 qed
+
+
+lemma rank_mon_refine:
+  shows "(rank_mon, (\<lambda> ballot a. RETURN (rank_l ballot a)))\<in> Id \<rightarrow> Id \<rightarrow> \<langle>Id\<rangle>nres_rel"
+  apply (refine_vcg rank_mon_correct)
+  apply simp
+  done
     
 
 section \<open>Monadic implementation of counting functions \<close>
@@ -114,9 +127,9 @@ text \<open>
   win-count, multiple refinement steps
 \<close>
 
-definition "wc_invar p0 a \<equiv> \<lambda>(r,ac).
-  r \<le> length p0 
-  \<and> ac = card{i::nat. i < r \<and> above (p0!i) a = {a}}"
+definition "wc_invar p0 a \<equiv> \<lambda>(i,ac).
+  i \<le> length p0 
+  \<and> ac = card{idx::nat. idx < i\<and> above (p0!idx) a = {a}}"
 
 definition win_count_mon :: "'a Profile \<Rightarrow> 'a \<Rightarrow> nat nres" where
 "win_count_mon p a \<equiv> do {
@@ -132,11 +145,14 @@ definition win_count_mon :: "'a Profile \<Rightarrow> 'a \<Rightarrow> nat nres"
 
 definition win_count_mon_r :: "'a Profile \<Rightarrow> 'a \<Rightarrow> nat nres" where
 "win_count_mon_r p a \<equiv> do {
-  (r, ac) \<leftarrow> WHILET (\<lambda>(r, _). r < length p) (\<lambda>(r, ac). do {
-    ASSERT (r < length p);
-    let ac = ac + (if (rank (p!r) a = 1) then 1 else 0);
-    let r = r + 1;
-    RETURN (r, ac)
+  (i, ac) \<leftarrow> WHILEIT (wc_invar p a) (\<lambda>(i, _). i < length p) (\<lambda>(i, ac). do {
+    ASSERT (i < length p);
+    let ballot = p!i;
+    let ranka = rank ballot a;
+    let wins = (if (ranka = 1) then 1 else 0);
+    let ac = ac + wins;
+    let i = i + 1;
+    RETURN (i, ac)
   })(0,0);
   RETURN ac
 }"
@@ -184,12 +200,17 @@ lemma carde: assumes pprofile: "profile A p"
   shows "\<forall> r < length p. (card (above (p ! r) a) = 1) = (above (p ! r) a = {a})" 
   using pprofile
     by (metis profile_def rank.simps Preference_Relation.rankone1 Preference_Relation.rankone2)
-    
+
+lemma isp1_measure: "wf (measure (\<lambda>(i, _).(length p) - i))" by simp
+
+lemma lgt0: "\<forall>l i. (i < length l \<longrightarrow> lengthl - Suc i < length l - i)"
+  oops
+
 lemma win_count_mon_r_correct:
   assumes prof: "profile A p"
   shows "win_count_mon_r p a \<le> SPEC (\<lambda> wc. wc = win_count p a)"
   unfolding win_count_mon_r_def win_count.simps
-  apply (intro WHILET_rule[where I="(wc_invar p a)" and R="measure (\<lambda>(r,_). (length p) - r)"] refine_vcg)
+  apply (intro WHILEIT_rule[where R="measure (\<lambda>(r,_). (length p) - r)"] refine_vcg)
   unfolding wc_invar_def
   apply (simp_all)
   apply (erule subst)
@@ -228,30 +249,18 @@ next
     by simp
 qed
 
+lemma win_count_mon_r_refine_spec:
+  shows "(win_count_mon_r, (\<lambda> p a. (RETURN (win_count p a)))) 
+    \<in> (br (\<lambda>x. x) (profile A)) \<rightarrow> Id \<rightarrow> \<langle>Id\<rangle>nres_rel"
+  apply (refine_vcg win_count_mon_r_correct) 
+  apply (auto simp add: refine_rel_defs)
+  done
+
+
 definition winsr :: "'a Preference_Relation \<Rightarrow> 'a \<Rightarrow> nat" where
   "winsr r a \<equiv> (if (rank r a = 1) then 1 else 0)"
 
-definition win_count_mon_outer :: "'a Profile \<Rightarrow> 'a \<Rightarrow> nat nres" where
-"win_count_mon_outer p a \<equiv> do {
-  (r, ac) \<leftarrow> WHILET (\<lambda>(r, _). r < length p) (\<lambda>(r, ac). do {
-    ASSERT (r < length p);
-    let ac = ac + winsr (p!r) a;
-    let r = r + 1;
-    RETURN (r, ac)
-  })(0,0);
-  RETURN ac
-}"
 
-lemma win_count_mon_outer_correct:
-  assumes prof: "profile A p"
-  shows "win_count_mon_outer p a \<le> SPEC (\<lambda> wc. wc = win_count p a)"
-proof -
-  have eq: "win_count_mon_outer p a = win_count_mon_r p a"
-  unfolding win_count_mon_outer_def win_count_mon_r_def winsr_def
-  by fastforce
-  from eq show ?thesis using win_count_mon_r_correct
-    using prof by fastforce 
-qed
 
 schematic_goal wc_code_aux: "RETURN ?wc_code \<le> win_count_mon p a"
   unfolding win_count_mon_def
@@ -272,13 +281,16 @@ export_code win_count in Scala
 
 text \<open> Data refinement \<close>
 
-definition winsr_imp :: "'a Preference_List \<Rightarrow> 'a \<Rightarrow> nat" where
-  "winsr_imp l a \<equiv> (if (rank_l l a = 1) then 1 else 0)"
+definition winsr_list :: "'a Preference_List \<Rightarrow> 'a \<Rightarrow> nat" where
+  "winsr_list l a \<equiv> (if (rank_l l a = 1) then 1 else 0)"
 
 (* This implementation requires the aasumption that ballots are not empty
    For empty ballots, a guard must be added to avoid accessing the first element *)
-definition winsr_imp' :: "'a Preference_List \<Rightarrow> 'a \<Rightarrow> nat" where
-  "winsr_imp' l a \<equiv> (if ((length l > 0) \<and> (l!0 = a)) then 1 else 0)"
+definition winsr_imp' :: "'a Preference_List \<Rightarrow> 'a \<Rightarrow> nat nres" where
+  "winsr_imp' l a \<equiv> do {
+    ranka \<leftarrow> rank_mon l a;
+    RETURN (if (ranka = 1) then 1 else 0)
+}"
 
 (* these auxiliary lemmas illustrate the equivalence of checking the the first
   candidate on a non empty ballot. *)
@@ -286,7 +298,7 @@ lemma top_above:
   assumes ne: "length pl > 0"
   shows "pl!0 = a \<longleftrightarrow> above_l pl a = [a]"
   unfolding above_l_def
-proof (auto)
+proof (simp add: rankdef, safe)
   assume mem: "List.member pl (pl ! 0)"
   assume "a = pl ! 0"
   have "List_Index.index pl (pl ! 0) = 0"
@@ -322,23 +334,24 @@ proof -
 qed
 
 
-lemma winsr_imp_refine:
+lemma winsr_list_refine:
   assumes "(l,r)\<in>build_rel pl_\<alpha> (ballot_on A)" and aA: "a \<in> A"
-  shows "winsr_imp l a = (winsr r a)"
-  unfolding winsr_imp_def winsr_def
-  using rankeq
-  by (metis assms in_br_conv)
+  shows "winsr_list l a = (winsr r a)"
+  unfolding winsr_list_def winsr_def
+  using rankeq assms
+  by (metis in_br_conv)
 
 lemma nmem_empty_l[simp]:
   shows "\<not>List.member [] a"
     by (simp add: member_rec(2))
 
-lemma winsr_imp'_eq:
-  assumes "well_formed_pl l" 
+lemma winsr_imp'_ref:
 (*and "l \<noteq> []"  necessary when not checking for empty ballots *)
-  shows "winsr_imp' l a = (winsr_imp l a)"
-  unfolding winsr_imp'_def winsr_imp_def
-proof (simp, safe)
+  shows "(winsr_imp', (\<lambda> ballot a. RETURN (winsr_list ballot a))) \<in> Id \<rightarrow> Id \<rightarrow> \<langle>Id\<rangle>nres_rel"
+  unfolding winsr_imp'_def winsr_list_def
+  apply (refine_vcg rank_mon_correct)
+  by auto
+(*proof (auto)
   show "List_Index.index l (l ! 0) = 0"
     by (simp add: index_eqI) 
 next
@@ -350,83 +363,146 @@ next
   assume "\<not> List.member l (l ! 0)" and "l \<noteq> []"
   thus "False"
     by (metis hd_conv_nth hd_in_set in_set_member)
-qed
+qed*)
 
 
 definition win_count_imp :: "'a Profile_List \<Rightarrow> 'a \<Rightarrow> nat nres" where
 "win_count_imp p a \<equiv> do {
-  (r, ac) \<leftarrow> WHILET (\<lambda>(r, _). r < length p) (\<lambda>(r, ac). do {
-    ASSERT (r < length p);
-    let ac = ac + (winsr_imp (p!r) a);
-    let r = r + 1;
-    RETURN (r, ac)
-  })(0,0);
-  RETURN ac
-}"
-  
-
-lemma win_count_imp_refine: 
-  assumes "(pl,pr)\<in>br pl_to_pr_\<alpha> (profile_l A)" and aA: "a \<in> A"
-  shows "win_count_imp pl a \<le> \<Down>Id (win_count_mon_outer pr a)"
-  using assms unfolding win_count_imp_def win_count_mon_outer_def pl_to_pr_\<alpha>_def
-  apply (refine_rcg)
-  apply (refine_dref_type) \<comment> \<open>Type-based heuristics to instantiate data 
-    refinement goals\<close>
-      apply (auto simp add: refine_rel_defs )
-  by (metis profile_l_def rankeq winsr_def winsr_imp_def)
-  
-    
-theorem win_count_imp_correct:
-  assumes "(pl,pr)\<in>build_rel pl_to_pr_\<alpha> (profile_l A)" and aA: "a \<in> A"
-  shows "win_count_imp pl a \<le> SPEC (\<lambda> wc. wc = win_count pr a)"
-  using ref_two_step[OF win_count_imp_refine win_count_mon_outer_correct] assms
-    profile_data_refine by fastforce
-  
-  
-definition win_count_imp' :: "'a Profile_List \<Rightarrow> 'a \<Rightarrow> nat nres" where
-"win_count_imp' p a \<equiv> do {
-  (r, ac) \<leftarrow> WHILET (\<lambda>(r, _). r < length p) (\<lambda>(r, ac). do {
-    ASSERT (r < length p);
-    let ac = ac + (winsr_imp' (p!r) a);
-    let r = r + 1;
-    RETURN (r, ac)
+  (i, ac) \<leftarrow> WHILET (\<lambda>(i, _). i < length p) (\<lambda>(i, ac). do {
+    ASSERT (i < length p);
+    let ballot = p!i;
+    let ranka = rank_l ballot a;
+    let wins = (if (ranka = 1) then 1 else 0);
+    let ac = ac + wins;
+    let i = i + 1;
+    RETURN (i, ac)
   })(0,0);
   RETURN ac
 }"
 
-
-lemma win_count_imp'_refine: 
-  fixes a:: "'a"
-  assumes "profile_l A pl"
-  shows "win_count_imp' pl a \<le> \<Down>Id (win_count_imp pl a)"
-  unfolding win_count_imp'_def win_count_imp_def wc_invar_def
-  apply (refine_rcg)
-  apply (refine_dref_type) \<comment> \<open>Type-based heuristics to instantiate data 
-    refinement goals\<close>
-  apply clarsimp_all
-proof (unfold winsr_imp'_def winsr_imp_def, (simp_all add: index_eqI), safe)
-  fix x1
-  assume range: "x1 < length pl"
-  assume mem: "List.member (pl ! x1) a"
-  assume nfst: "(pl!x1!0) \<noteq> a"
-  from range mem nfst show "List_Index.index (pl ! x1) a > 0"
-    by (metis in_set_member nth_index zero_less_iff_neq_zero)
-next
-  fix x1
-  assume range: "x1 < length pl"
-  assume nmem: "\<not> List.member (pl ! x1) (pl ! x1 ! 0)"
-  assume "pl ! x1 \<noteq> []"
-  from nmem this show "False" by (metis hd_conv_nth hd_in_set in_set_member)
+lemma rankeq_refine: 
+  fixes A :: "'a set" and l :: "'a Preference_List" and a :: 'a
+  assumes "(pl, pr) \<in> (br pl_\<alpha> (ballot_on A))"
+  shows "rank_l pl a = Preference_Relation.rank pr a"
+proof -
+  from assms have ballot: "ballot_on A pl" using in_br_conv
+    by metis
+  from assms have "pr = pl_\<alpha> pl"
+    by (simp add: in_br_conv)
+  from ballot this show ?thesis using rankeq
+    by metis
 qed
 
 
-theorem win_count_imp'_correct:
-  assumes "(pl,pr)\<in>build_rel pl_to_pr_\<alpha> (profile_l A)" and aA: "a \<in> A"
-  shows "win_count_imp' pl a \<le> SPEC (\<lambda> wc. wc = win_count pr a)"
-  using ref_two_step[OF win_count_imp'_refine win_count_imp_correct] 
-      assms refine_IdD in_br_conv
-  by metis
+lemma win_count_imp_refine: 
+  shows "(win_count_imp, win_count_mon_r) \<in> (br pl_to_pr_\<alpha> (profile_l A)) \<rightarrow> Id \<rightarrow> \<langle>Id\<rangle>nres_rel"
+  unfolding win_count_imp_def win_count_mon_r_def pl_to_pr_\<alpha>_def profile_l_def
+  apply (refine_vcg rankeq_refine)
+      apply clarsimp_all
+  apply (refine_dref_type) \<comment> \<open>Type-based heuristics to instantiate data 
+    refinement goals\<close>
+  apply (auto simp add: rankeq_refine refine_rel_defs)
+proof (-)
+  fix pl:: "'a Profile_List"
+  fix idx::nat
+  fix alt::'a
+  assume prof: "\<forall>i<length pl. ballot_on A (pl ! i)"
+  assume ir: "idx < length pl"
+  assume con: "alt \<in> set (pl ! idx)"
+  assume fst: "index (pl ! idx) alt = 0"
+  from prof ir have ibal: "ballot_on A (pl!idx)"
+    by blast 
+  from ibal con have aA: "alt \<in> A"
+    by (metis Preference_List.limited_def connex_l_def in_set_member lin_ord_imp_connex_l)
+  from con fst have "(rank_l (pl!idx) alt) = 1"
+    by auto
+  from aA ibal this have "(rank (pl_\<alpha> (pl!idx)) alt) = 1" using rankeq
+    by metis
+  from this show "card (above (pl_\<alpha> (pl!idx)) alt) = Suc 0"
+    by simp
+next
+ fix pl:: "'a Profile_List"
+  fix idx::nat
+  fix alt::'a
+  assume prof: "\<forall>i<length pl. ballot_on A (pl ! i)"
+  assume ir: "idx < length pl"
+  assume con: "alt \<in> set (pl ! idx)"
+  assume fst: "index (pl ! idx) alt > 0"
+  assume np: "card (above (pl_\<alpha> (pl ! idx)) alt) = Suc 0"
+  from prof ir have ibal: "ballot_on A (pl!idx)"
+    by blast 
+  from ibal con have aA: "alt \<in> A"
+    by (metis Preference_List.limited_def connex_l_def in_set_member lin_ord_imp_connex_l)
+  from con fst have "(rank_l (pl!idx) alt) > 1"
+    by auto
+  from ibal this have "(rank (pl_\<alpha> (pl!idx)) alt) > 1" using rankeq
+    by metis
+  from this np show "False" by simp
+next
+  fix pl:: "'a Profile_List"
+  fix idx::nat
+  fix alt::'a
+  assume prof: "\<forall>i<length pl. ballot_on A (pl ! i)"
+  assume ir: "idx < length pl"
+  assume ncon: "alt \<notin> set (pl ! idx)"
+  assume rank1: "card (above (pl_\<alpha> (pl ! idx)) alt) = Suc 0"
+  from prof ir have ibal: "ballot_on A (pl!idx)"
+    by blast 
+  from ncon have "rank_l (pl!idx) alt = 0"
+    by simp 
+  from ibal this have "rank (pl_\<alpha> (pl ! idx)) alt = 0"
+    using rankeq
+    by metis
+  from this rank1 show "False"
+    by simp
+qed
+  
+theorem win_count_imp_correct:
+  shows "(win_count_imp, (\<lambda> pr a. RETURN (win_count pr a))) \<in>
+    br pl_to_pr_\<alpha> (profile_l A) \<rightarrow> Id \<rightarrow> \<langle>Id\<rangle>nres_rel"
+  apply (refine_vcg win_count_imp_refine win_count_mon_r_refine_spec)
+proof auto
+  fix pl:: "'a Profile_List"
+  fix pr:: "'a Profile"
+  fix alt:: 'a
+  assume rel: "(pl, pr) \<in> br pl_to_pr_\<alpha> (profile_l A)"
+  from this have "profile_l A pl" using in_br_conv by metis
+  from rel this have "profile A pr"
+    using profile_data_refine by blast
+  from this have "win_count_mon_r pr alt \<le> SPEC (\<lambda>c. (c, win_count pr alt) \<in> nat_rel)"
+    using win_count_mon_r_correct by (metis (mono_tags, lifting) SPEC_cons_rule pair_in_Id_conv)
+  from this 
+    rel have "win_count_imp pl alt \<le> SPEC (\<lambda>c. (c, win_count pr alt) \<in> nat_rel)" using win_count_imp_refine
+    by (metis conc_trans_additional(5) nres_relD pair_in_Id_conv relAPP_def tagged_fun_relD_both)
+  from this show "win_count_imp pl alt \<le> RES {card {i. i < length pr \<and> above (pr ! i) alt = {alt}}}"
+    by fastforce
+qed
+  
 
+
+definition win_count_r_imp :: "'a Profile_List \<Rightarrow> 'a \<Rightarrow> nat nres" where
+"win_count_r_imp p a \<equiv> do {
+  (i, ac) \<leftarrow> WHILET (\<lambda>(i, _). i < length p) (\<lambda>(i, ac). do {
+    ASSERT (i < length p);
+    let ballot = p!i;
+    ranka \<leftarrow> (rank_mon ballot a);
+    let ac = ac + (if (ranka = 1) then 1 else 0);
+    let i = i + 1;
+    RETURN (i, ac)
+  })(0,0);
+  RETURN ac
+}"
+
+lemma win_count_imp_r_refine: 
+  shows "(win_count_r_imp, win_count_imp) \<in> Id \<rightarrow> Id \<rightarrow> \<langle>Id\<rangle>nres_rel"
+  unfolding win_count_r_imp_def win_count_imp_def
+  apply (refine_vcg rank_mon_correct)
+  apply (refine_dref_type) \<comment> \<open>Type-based heuristics to instantiate data 
+    refinement goals\<close>
+  apply (auto simp add: refine_rel_defs)
+  done
+
+(* TODO correctness proof *)
 
 text \<open>
   pref count
