theories/Compositional_Structures/Basic_Modules/Component_Types/Social_Choice_Types/Profile_Sepref.thy
@@ -11,23 +11,49 @@ definition "ballot_rel A \<equiv> br pl_\<alpha> (ballot_on A)"
 
 definition "ballot_assn A \<equiv> hr_comp (array_assn id_assn) (ballot_rel A)"
 
-abbreviation "cand_assn \<equiv> (id_assn::'a \<Rightarrow> _)"
+abbreviation "cand_assn \<equiv> (id_assn::(nat) \<Rightarrow> _)"
 
 
 sepref_definition idx_imp is 
   "uncurry index_mon" :: "(array_assn nat_assn)\<^sup>k *\<^sub>a (nat_assn)\<^sup>k \<rightarrow>\<^sub>a nat_assn"
   unfolding index_mon_def[abs_def] index_mon_inv_def[abs_def]
+  by sepref 
+(* supply [[goals_limit = 1]]
+  apply sepref_dbg_keep
+  apply sepref_dbg_trans_keep \<comment> \<open>(1) We get stuck at an equals operation\<close>
+  apply sepref_dbg_trans_step_keep
+ *)
+
+
+
+(*export_code idx_imp in OCaml_imp module_name IndexCompute*)
+
+thm idx_imp.refine
+
+lemmas idx_imp_correct = idx_imp.refine[FCOMP index_mon_refine]
+
+sepref_definition rank_imp is
+  "uncurry rank_mon" :: "(array_assn nat_assn)\<^sup>k *\<^sub>a (nat_assn)\<^sup>k \<rightarrow>\<^sub>a nat_assn"
+  unfolding rank_mon_def[abs_def] index_mon_def[abs_def] index_mon_inv_def[abs_def]
   by sepref
-  
+
+lemmas rank_imp_correct = rank_imp.refine[FCOMP rank_mon_refine]
 
 
 definition "profile_rel A \<equiv> br pl_to_pr_\<alpha> (profile_l A)"
 
-
-
-abbreviation "profile_impl_assn \<equiv> array_assn (array_assn id_assn)"
+abbreviation "profile_impl_assn \<equiv> array_assn (array_assn nat_assn)"
 
 definition "profile_assn A
     \<equiv> hr_comp profile_impl_assn (profile_rel A)"
+
+sepref_definition win_count_imp_sep is
+  "uncurry win_count_imp" :: "(profile_impl_assn)\<^sup>k *\<^sub>a (nat_assn)\<^sup>k \<rightarrow>\<^sub>a nat_assn"
+  unfolding win_count_imp_def[abs_def] 
+    rank_mon_def[abs_def]
+  apply sepref_dbg_keep
+      apply sepref_dbg_trans_keep
+ apply sepref_dbg_trans_step_keep
+
 
 end
